Checkpoint... Notation madness.

src/rocq/Handlers/MemoryModel.v
@@ -5,6 +5,10 @@ From Vellvm.Syntax Require Import
      DataLayout
      DynamicTypes.
 
+Unset Universe Checking.
+From CTree Require Import
+  CTree Eq.
+
 From ITree Require Import
      ITree
      Basics.Basics
@@ -30,6 +34,7 @@ From Vellvm.Handlers Require Import
   MemPropT
   MemoryModules.Within.
 
+Unset Universe Checking.
 From Vellvm.Utils Require Import
      Error
      PropT
@@ -42,7 +47,9 @@ From Vellvm.Utils Require Import
      MonadReturnsLaws
      MonadEq1Laws
      MonadExcLaws
-     Inhabited.
+     Inhabited
+     CTreeUtils
+     RaiseCtree.
 
 From ExtLib Require Import
      Structures.Monads
@@ -72,6 +79,8 @@ Import EitherMonad.
 
 From Stdlib Require Import FunctionalExtensionality.
 Import Logic.
+
+Open Scope N.
 
 Module Type MemoryModelSpecPrimitives (LP : LLVMParams) (MP : MemoryParams LP).
   Import LP.Events.
@@ -1042,7 +1051,7 @@ Module MemoryHelpers (LP : LLVMParams) (MP : MemoryParams LP) (Byte : ByteModule
             unfold sequence in Heqo.
 
             eapply map_monad_OOM_Nth with (n:=n) in Heqo as [pa [EQPA NTH_pa]].
-            unfold id in EQPA. inv EQPA.
+            unfold Datatypes.id in EQPA. inv EQPA.
             eapply NTH_pa.
             eapply PTRS_n.
           }
@@ -1299,7 +1308,7 @@ Module MemoryHelpers (LP : LLVMParams) (MP : MemoryParams LP) (Byte : ByteModule
             unfold sequence in Heqo.
 
             eapply map_monad_OOM_Nth with (n:=n) in Heqo as [pa [EQPA NTH_pa]].
-            unfold id in EQPA. inv EQPA.
+            unfold Datatypes.id in EQPA. inv EQPA.
             eapply NTH_pa.
             eapply PTRS_n.
           }
@@ -1768,7 +1777,7 @@ Module MemoryHelpers (LP : LLVMParams) (MP : MemoryParams LP) (Byte : ByteModule
     pose proof HSEQUENCE.
     eapply map_monad_OOM_Nth in HSEQUENCE; eauto.
     destruct HSEQUENCE as [y [EQY NTHY]].
-    unfold id in EQY; inv EQY.
+    unfold Datatypes.id in EQY; inv EQY.
 
     eapply map_monad_err_Nth in MAP as [ix [P NTH']]; eauto.
     exists ix; split; eauto.
@@ -3100,13 +3109,13 @@ Module Type MemoryModelSpec (LP : LLVMParams) (MP : MemoryParams LP) (MMSP : Mem
       (* Bytes not allocated in the popped frame have the same allocation status as before *)
       non_frame_bytes_preserved :
       forall ptr aid,
-        (~ ptr_in_current_frame m1 ptr) ->
+        ~ ptr_in_current_frame m1 ptr ->
         byte_allocated m1 ptr aid <-> byte_allocated m2 ptr aid;
 
       (* Bytes not allocated in the popped frame are the same when read *)
       non_frame_bytes_read :
       forall ptr byte,
-        (~ ptr_in_current_frame m1 ptr) ->
+        ~ ptr_in_current_frame m1 ptr ->
         read_byte_spec m1 ptr byte <-> read_byte_spec m2 ptr byte;
 
       (* Set new framestack *)
@@ -3261,7 +3270,15 @@ Module Type MemoryModelSpec (LP : LLVMParams) (MP : MemoryParams LP) (MMSP : Mem
 
   (*** Allocation utilities *)
   Record block_is_free (m1 : MemState) (len : nat) (pr : Provenance) (ptr : addr) (ptrs : list addr) : Prop :=
-    { block_is_free_consecutive : ret ptrs {{m1}} ∈ {{m1}} get_consecutive_ptrs ptr len;
+    { block_is_free_consecutive : 
+      @within (MemPropT MemState) (@MemPropT_Eq1 MemState) err_ub_oom MemState MemState
+        (@Within_err_ub_oom_MemPropT MemState) (list addr)
+        (@get_consecutive_ptrs (MemPropT MemState) (@MemPropT_Monad MemState)
+           (@MemPropT_RAISE_OOM MemState) (@MemPropT_RAISE_ERROR MemState) ptr len)
+        m1
+        (@ret err_ub_oom (@Monad_err_ub_oom IdentityMonad.ident IdentityMonad.Monad_ident)
+           (list addr) ptrs)
+        m1; (* ret ptrs {{m1}} ∈ {{m1}} get_consecutive_ptrs ptr len; *)
       block_is_free_ptr_provenance : address_provenance ptr = allocation_id_to_prov (provenance_to_allocation_id pr); (* Need this case if `ptrs` is empty (allocating 0 bytes) *)
       block_is_free_ptrs_provenance : forall ptr, In ptr ptrs -> address_provenance ptr = allocation_id_to_prov (provenance_to_allocation_id pr);
 
@@ -3529,13 +3546,13 @@ Module Type MemoryModelSpec (LP : LLVMParams) (MP : MemoryParams LP) (MMSP : Mem
       (* Bytes not allocated in the block have the same allocation status as before *)
       free_non_block_bytes_preserved :
       forall ptr aid,
-        (~ ptr_in_memstate_heap m1 root ptr) ->
+        ~ ptr_in_memstate_heap m1 root ptr ->
         byte_allocated m1 ptr aid <-> byte_allocated m2 ptr aid;
 
       (* Bytes not allocated in the freed block are the same when read *)
       free_non_frame_bytes_read :
       forall ptr byte,
-        (~ ptr_in_memstate_heap m1 root ptr) ->
+        ~ ptr_in_memstate_heap m1 root ptr ->
         read_byte_spec m1 ptr byte <-> read_byte_spec m2 ptr byte;
 
       (* Set new heap *)
@@ -3666,7 +3683,7 @@ Module Type MemoryModelSpec (LP : LLVMParams) (MP : MemoryParams LP) (MMSP : Mem
       refine
         (match args with
          | DVALUE_Addr dst ::
-             @DVALUE_I sz_val val ::
+             @DVALUE_I sz_val value ::
              @DVALUE_I sz_len len ::
              @DVALUE_I sz_vol volatile :: [] (* volatile ignored *)  =>
              _
@@ -3676,7 +3693,7 @@ Module Type MemoryModelSpec (LP : LLVMParams) (MP : MemoryParams LP) (MMSP : Mem
       destruct (Pos.eq_dec sz_val 8); subst.
       - exact
           (sid <- fresh_sid;;
-           memset_spec dst val (unsigned len) sid (equ volatile VellvmIntegers.one)).
+           memset_spec dst value (unsigned len) sid (equ volatile VellvmIntegers.one)).
       - exact (raise_error "Unsupported arguments to memset.").
     Defined.
 
@@ -4301,20 +4318,42 @@ Module Type MemoryExecMonad (LP : LLVMParams) (MP : MemoryParams LP) (MMSP : Mem
 
   Definition within_err_ub_oom_itree
     {Pre Post : Type}
-    {Eff}
+    {Eff B}
     `{FAIL : FailureE -< Eff} `{UB : UBE -< Eff} `{OOM : OOME -< Eff}
-    {A} (t : itree Eff A) (pre : Pre) (e : err_ub_oom A) (post : Post) : Prop :=
-    t ≈ lift_err_ub_oom ret e.
+    {X} (t : ctree Eff B X) (pre : Pre) (e : err_ub_oom X) (post : Post) : Prop :=
+    t ~ @lift_err_ub_oom_ctree X X Eff B _ _ _ ret e.
 
   (* Version that uses RAISE_OOM etc explicitly *)
   Import IdentityMonad.
   Definition within_err_ub_oom_itree'
     {Pre Post : Type}
-    {Eff}
-    `{EQI : Eq1 (itree Eff)}
-    `{MITREE : Monad (itree Eff)}
-    `{FAIL : RAISE_ERROR (itree Eff)} `{UB : RAISE_UB (itree Eff)} `{OOM : RAISE_OOM (itree Eff)}
-    {A} (t : itree Eff A) (pre : Pre) (e : err_ub_oom A) (post : Post) : Prop :=
+    {Eff B}
+    `{EQI : Eq1 (ctree Eff B)}
+    `{MITREE : Monad (ctree Eff B)}
+    `{FAIL : RAISE_ERROR (ctree Eff B)} `{UB : RAISE_UB (ctree Eff B)} `{OOM : RAISE_OOM (ctree Eff B)}
+    {A} (t : ctree Eff B A) (pre : Pre) (e : err_ub_oom A) (post : Post) : Prop :=
+    match e with
+    | ERR_UB_OOM (mkEitherT (mkEitherT (mkEitherT (mkIdent m)))) =>
+        match m with
+        | inl (OOM_message x) =>
+            exists oom_msg, (t ≈ raise_oom oom_msg)%monad
+        | inr (inl (UB_message x)) =>
+            (* Should this be more permissive? *)
+            exists ub_msg, (t ≈ raise_ub ub_msg)%monad
+        | inr (inr (inl (ERR_message x))) =>
+            exists err_msg, (t ≈ raise_error err_msg)%monad
+        | inr (inr (inr x)) =>
+            (t ≈ ret x)%monad
+        end
+    end.
+
+  Definition within_err_ub_oom_ctree'
+    {Pre Post : Type}
+    {Eff B}
+    `{EQI : Eq1 (ctree Eff B)}
+    `{MITREE : Monad (ctree Eff B)}
+    `{FAIL : RAISE_ERROR (ctree Eff B)} `{UB : RAISE_UB (ctree Eff B)} `{OOM : RAISE_OOM (ctree Eff B)}
+    {A} (t : ctree Eff B A) (pre : Pre) (e : err_ub_oom A) (post : Post) : Prop :=
     match e with
     | ERR_UB_OOM (mkEitherT (mkEitherT (mkEitherT (mkIdent m)))) =>
         match m with
@@ -4332,10 +4371,10 @@ Module Type MemoryExecMonad (LP : LLVMParams) (MP : MemoryParams LP) (MMSP : Mem
 
   Lemma within_Proper_err_ub_oom_itree
     {Pre Post : Type}
-    {Eff}
+    {Eff B}
     `{FAIL : FailureE -< Eff} `{UB : UBE -< Eff} `{OOM : OOME -< Eff}
-    {A} :
-    Proper (eq1 ==> eq ==> eq ==> eq ==> iff) (within_err_ub_oom_itree (Eff:=Eff) (Pre:=Pre) (Post:=Post) (A:=A)).
+    {X} :
+    Proper (eq1 ==> eq ==> eq ==> eq ==> iff) (within_err_ub_oom_itree (Eff:=Eff) (B:=B) (Pre:=Pre) (Post:=Post) (X:=X)).
   Proof.
     unfold Proper, respectful.
     intros x y H x0 y0 H0 x1 y1 H1 x2 y2 H2.
@@ -4350,11 +4389,11 @@ Module Type MemoryExecMonad (LP : LLVMParams) (MP : MemoryParams LP) (MMSP : Mem
 
   Lemma within_Proper_err_ub_oom_itree'
     {Pre Post : Type}
-    {Eff}
-    `{EQI : Eq1 (itree Eff)}
-    `{MITREE : Monad (itree Eff)}
-    `{EQV : @Eq1Equivalence (itree Eff) _ EQI}
-    `{FAIL : RAISE_ERROR (itree Eff)} `{UB : RAISE_UB (itree Eff)} `{OOM : RAISE_OOM (itree Eff)}
+    {Eff B}
+    `{EQI : Eq1 (ctree Eff B)}
+    `{MITREE : Monad (ctree Eff B)}
+    `{EQV : @Eq1Equivalence (ctree Eff B) _ EQI}
+    `{FAIL : RAISE_ERROR (ctree Eff B)} `{UB : RAISE_UB (ctree Eff B)} `{OOM : RAISE_OOM (ctree Eff B)}
     {A} :
     Proper (eq1 ==> eq ==> eq ==> eq ==> iff) (within_err_ub_oom_itree' (EQI:=EQI) (Pre:=Pre) (Post:=Post) (A:=A)).
   Proof.
@@ -4371,14 +4410,35 @@ Module Type MemoryExecMonad (LP : LLVMParams) (MP : MemoryParams LP) (MMSP : Mem
         auto.
   Qed.
 
+  Lemma within_Proper_err_ub_oom_ctree'
+    {Pre Post : Type}
+    {Eff B}
+    `{EQI : Eq1 (ctree Eff B)}
+    `{EQV : @Eq1Equivalence (ctree Eff B) _ EQI}
+    `{FAIL : RAISE_ERROR (ctree Eff B)} `{UB : RAISE_UB (ctree Eff B)} `{OOM : RAISE_OOM (ctree Eff B)}
+    {A} :
+    Proper (eq1 ==> eq ==> eq ==> eq ==> iff) (within_err_ub_oom_ctree' (EQI:=EQI) (Pre:=Pre) (Post:=Post) (A:=A)).
+  Proof.
+    unfold Proper, respectful.
+    intros x y H x0 y0 H0 x1 y1 H1 x2 y2 H2.
+    subst.
+    unfold within_err_ub_oom_ctree' in *.
+    split; intros WITHIN.
+    - destruct y1 as [[[[[[[oom_y1] | [[ub_y1] | [[err_y1] | y1']]]]]]]] eqn:Hy1;
+        setoid_rewrite H in WITHIN;
+        auto.
+    - destruct y1 as [[[[[[[oom_y1] | [[ub_y1] | [[err_y1] | y1']]]]]]]] eqn:Hy1;
+        setoid_rewrite H;
+        auto.
+  Qed.
+
   #[global] Instance Within_err_ub_oom_itree'
     {Pre Post : Type}
-    {Eff}
-    `{EQI : Eq1 (itree Eff)}
-    `{MITREE : Monad (itree Eff)}
-    `{EQV : @Eq1Equivalence (itree Eff) _ EQI}
-    `{FAIL : RAISE_ERROR (itree Eff)} `{UB : RAISE_UB (itree Eff)} `{OOM : RAISE_OOM (itree Eff)}
-    : @Within (itree Eff) _ err_ub_oom Pre Post.
+    {Eff B}
+    `{EQI : Eq1 (ctree Eff B)}
+    `{EQV : @Eq1Equivalence (ctree Eff B) _ EQI}
+    `{FAIL : RAISE_ERROR (ctree Eff B)} `{UB : RAISE_UB (ctree Eff B)} `{OOM : RAISE_OOM (ctree Eff B)}
+    : @Within (ctree Eff B) _ err_ub_oom Pre Post.
   Proof.
     esplit.
     intros A.
@@ -4387,16 +4447,46 @@ Module Type MemoryExecMonad (LP : LLVMParams) (MP : MemoryParams LP) (MMSP : Mem
     eapply within_Proper_err_ub_oom_itree'; eauto.
   Defined.
 
-  (* Should probably be derivable with typeclasses eauto... *)
-  #[global] Instance Within_err_ub_oom_MemM {MemM Eff}
-    `{EQI : Eq1 (itree Eff)}
-    `{MITREE : Monad (itree Eff)}
-    `{EQV : @Eq1Equivalence (itree Eff) _ EQI}
-    `{FAIL : RAISE_ERROR (itree Eff)} `{UB : RAISE_UB (itree Eff)} `{OOM : RAISE_OOM (itree Eff)}
-    `{MM: MemMonad MemM (itree Eff)} : @Within MemM _ err_ub_oom (store_id * MemState)%type (store_id * MemState)%type.
+  #[global] Instance Within_err_ub_oom_ctree'
+    {Pre Post : Type}
+    {Eff B}
+    `{EQI : Eq1 (ctree Eff B)}
+    `{EQV : @Eq1Equivalence (ctree Eff B) _ EQI}
+    `{FAIL : RAISE_ERROR (ctree Eff B)} `{UB : RAISE_UB (ctree Eff B)} `{OOM : RAISE_OOM (ctree Eff B)}
+    : @Within (ctree Eff B) EQI err_ub_oom Pre Post.
   Proof.
-    eapply @Transitive_Within with (M1:=err_ub_oom) (M2:=itree Eff) (M3:=MemM).
+    esplit.
+    intros A.
+    unfold Proper, respectful.
+    intros x y H x0 y0 H0 x1 y1 H1 x2 y2 H2; subst.
+    eapply (@within_Proper_err_ub_oom_ctree' Pre Post Eff B EQI EQV FAIL UB OOM); eauto.
+    Unshelve.
+    all: eauto.
+  Defined.
+
+
+  (* Should probably be derivable with typeclasses eauto... *)
+  #[global] Instance Within_err_ub_oom_MemM {MemM Eff B}
+    `{EQI : Eq1 (ctree Eff B)}
+    `{EQV : @Eq1Equivalence (ctree Eff B) _ EQI}
+    `{FAIL : RAISE_ERROR (ctree Eff B)} `{UB : RAISE_UB (ctree Eff B)} `{OOM : RAISE_OOM (ctree Eff B)}
+    `{MM: MemMonad MemM (ctree Eff B)} : @Within MemM _ err_ub_oom (store_id * MemState)%type (store_id * MemState)%type.
+  Proof.
+    eapply @Transitive_Within with (M1:=err_ub_oom) (M2:=ctree Eff B) (M3:=MemM).
     - eapply Within_err_ub_oom_itree'.
+    - eapply Within_RunM_MemMonad.
+  Defined.
+
+  (* Should probably be derivable with typeclasses eauto... *)
+  #[global] Instance Within_err_ub_oom_MemM_ctree {MemM Eff B}
+    `{EQI : Eq1 (ctree Eff B)}
+    `{EQV : @Eq1Equivalence (ctree Eff B) _ EQI}
+    `{FAIL : RAISE_ERROR (ctree Eff B)} `{UB : RAISE_UB (ctree Eff B)} `{OOM : RAISE_OOM (ctree Eff B)}
+    `{MM: MemMonad MemM (ctree Eff B)}
+    : @Within MemM _ err_ub_oom (store_id * MemState)%type (store_id * MemState)%type.
+  Proof.
+    eapply @Transitive_Within with (M1:=err_ub_oom) (M2:=ctree Eff B) (M3:=MemM).
+    - eapply Within_err_ub_oom_ctree'.
     - eapply Within_RunM_MemMonad.
   Defined.
 
@@ -4437,7 +4527,7 @@ Module Type MemoryExecMonad (LP : LLVMParams) (MP : MemoryParams LP) (MMSP : Mem
   #[global] Instance MonadStoreId_exec_correct_post : MonadStoreId exec_correct_post.
   split.
   refine (fun ms st sid ms' st' =>
-            sid <= st /\ st < st' /\ ms = ms').
+            sid <= st /\ st < st' /\ ms = ms')%N.
   Defined.
 
   #[global] Instance MonadProvenance_exec_correct_post : MonadProvenance Provenance exec_correct_post.
@@ -4574,7 +4664,7 @@ Module Type MemoryExecMonad (LP : LLVMParams) (MP : MemoryParams LP) (MMSP : Mem
     auto.
   Qed.
 
-  Definition exec_correct {MemM Eff} `{MM: MemMonad MemM (itree Eff)} {X} (pre : exec_correct_pre) (exec : MemM X) (spec : MemPropT MemState X) (post : exec_correct_post X) : Prop :=
+  Definition exec_correct {MemM Eff B} `{MM: MemMonad MemM (ctree Eff B)} {X} (pre : exec_correct_pre) (exec : MemM X) (spec : MemPropT MemState X) (post : exec_correct_post X) : Prop :=
     forall ms st,
       (MemMonad_valid_state ms st) ->
       pre ms st ->
@@ -4599,13 +4689,13 @@ Module Type MemoryExecMonad (LP : LLVMParams) (MP : MemoryParams LP) (MMSP : Mem
                  well, and if the executable returns successfully it
                  gives a valid store_id / MemState pair.
               *)
-             let WEM := (Within_err_ub_oom_MemM (EQI:=(@MemMonad_eq1_runm _ _ _ _ _ _ _ _ _ _ _ _ _ _ _ _ MM)) (EQV:=(@MemMonad_eq1_runm_equiv _ _ _ _ _ _ _ _ _ _ _ _ _ _ _ _ MM))) in
+             let WEM := (Within_err_ub_oom_MemM_ctree (EQI:=(@MemMonad_eq1_runm _ _ _ _ _ _ _ _ _ _ _ _ _ _ _ _ MM)) (EQV:=(@MemMonad_eq1_runm_equiv _ _ _ _ _ _ _ _ _ _ _ _ _ _ _ _ MM))) in
              (@within MemM _ err_ub_oom (store_id * MemState)%type (store_id * MemState)%type WEM X exec (st, ms) e (st', ms')) /\
                (e {{ms}} ∈ {{ms'}} spec) /\ ((exists x, e = ret x) -> (MemMonad_valid_state ms' st' /\ (exists x, e = ret x /\ post ms st x ms' st')))).
 
   (* TODO: Move this *)
   Lemma exec_correct_weaken_pre :
-    forall {MemM Eff} `{MEMM : MemMonad MemM (itree Eff)}
+    forall {MemM Eff B} `{MEMM : MemMonad MemM (ctree Eff B)}
       {A}
       (pre : exec_correct_pre)
       (post : exec_correct_post A)
@@ -4616,7 +4706,7 @@ Module Type MemoryExecMonad (LP : LLVMParams) (MP : MemoryParams LP) (MMSP : Mem
       exec_correct weak_pre exec spec post ->
       exec_correct pre exec spec post.
   Proof.
-    intros MemM Eff MM MRun MPROV MSID MMS MERR MUB MOOM RunERR RunUB RunOOM EQM EQRI MLAWS MEMM A pre post weak_pre exec spec WEAK EXEC.
+    intros MemM Eff B MM MRun MPROV MSID MMS MERR MUB MOOM RunERR RunUB RunOOM EQM EQRI MLAWS MEMM A pre post weak_pre exec spec WEAK EXEC.
     unfold exec_correct in *.
     intros ms st VALID PRE.
     apply WEAK in PRE.
@@ -4625,7 +4715,7 @@ Module Type MemoryExecMonad (LP : LLVMParams) (MP : MemoryParams LP) (MMSP : Mem
 
   (* TODO: Move this *)
   Lemma exec_correct_strengthen_post :
-    forall {MemM Eff} `{MEMM : MemMonad MemM (itree Eff)}
+    forall {MemM Eff B} `{MEMM : MemMonad MemM (ctree Eff B)}
       {A}
       (pre : exec_correct_pre)
       (post : exec_correct_post A)
@@ -4636,7 +4726,7 @@ Module Type MemoryExecMonad (LP : LLVMParams) (MP : MemoryParams LP) (MMSP : Mem
       exec_correct pre exec spec strong_post ->
       exec_correct pre exec spec post.
   Proof.
-    intros MemM Eff MM MRun MPROV MSID MMS MERR MUB MOOM RunERR RunUB RunOOM EQM EQRI MLAWS MEMM A pre post strong_post exec spec STRONG EXEC.
+    intros MemM Eff B MM MRun MPROV MSID MMS MERR MUB MOOM RunERR RunUB RunOOM EQM EQRI MLAWS MEMM A pre post strong_post exec spec STRONG EXEC.
     unfold exec_correct in *.
     intros ms st VALID PRE.
     specialize (EXEC _ _ VALID PRE).
@@ -4657,13 +4747,13 @@ Module Type MemoryExecMonad (LP : LLVMParams) (MP : MemoryParams LP) (MMSP : Mem
 
   (* TODO: move this *)
   Lemma exec_correct_bind :
-    forall {MemM Eff} `{MEMM : MemMonad MemM (itree Eff)}
-      {A B}
+    forall {MemM Eff B} `{MEMM : MemMonad MemM (ctree Eff B)}
+      {X Y}
       (pre : exec_correct_pre)
-      (post_a : exec_correct_post A)
-      (post_b : A -> exec_correct_post B)
-      (m_exec : MemM A) (k_exec : A -> MemM B)
-      (m_spec : MemPropT MemState A) (k_spec : A -> MemPropT MemState B),
+      (post_a : exec_correct_post X)
+      (post_b : X -> exec_correct_post Y)
+      (m_exec : MemM X) (k_exec : X -> MemM Y)
+      (m_spec : MemPropT MemState X) (k_spec : X -> MemPropT MemState Y),
       exec_correct pre m_exec m_spec post_a ->
       (* This isn't true:
 
@@ -4693,207 +4783,222 @@ Module Type MemoryExecMonad (LP : LLVMParams) (MP : MemoryParams LP) (MMSP : Mem
                                                                                 (MemMonad_run m_exec ms_init st_init)
                                                                                 (ret (st_after_m, (ms_after_m, a))))%monad ->
           (* ms_k is a MemState after evaluating m *)
-          let WEM := (Within_err_ub_oom_MemM (EQI:=(@MemMonad_eq1_runm _ _ _ _ _ _ _ _ _ _ _ _ _ _ _ _ MEMM)) (EQV:=(@MemMonad_eq1_runm_equiv _ _ _ _ _ _ _ _ _ _ _ _ _ _ _ _ MEMM))) in
+          let WEM := (Within_err_ub_oom_MemM_ctree (EQI:=(@MemMonad_eq1_runm _ _ _ _ _ _ _ _ _ _ _ _ _ _ _ _ MEMM)) (EQV:=(@MemMonad_eq1_runm_equiv _ _ _ _ _ _ _ _ _ _ _ _ _ _ _ _ MEMM))) in
           exec_correct (fun ms_k st_k =>
                           pre ms_init st_init /\
                             (@within MemM _ err_ub_oom (store_id * MemState)%type (store_id * MemState)%type WEM _ m_exec (st_init, ms_init) (ret a) (st_k, ms_k))
                           /\ m_spec ms_init (ret (ms_k, a))) (k_exec a) (k_spec a) (post_b a)) ->
       exec_correct pre (a <- m_exec;; k_exec a) (a <- m_spec;; k_spec a) (a <- post_a;; post_b a).
   Proof.
-    intros MemM Eff MM MRun MPROV MSID MMS
-      MERR MUB MOOM RunERR RunUB RunOOM EQM EQRI
-      MLAWS MEMM A B pre post_a post_b m_exec k_exec m_spec
-      k_spec M_CORRECT K_CORRECT.
+    (* intros MemM Eff B MM MRun MPROV MSID MMS *)
+    (*   MERR MUB MOOM RunERR RunUB RunOOM EQM EQRI *)
+    (*   MLAWS MEMM X Y pre post_a post_b m_exec k_exec m_spec *)
+    (*   k_spec M_CORRECT K_CORRECT. *)
 
-    unfold exec_correct in *.
-    intros ms st VALID PRE.
-    specialize (M_CORRECT ms st VALID PRE).
-    destruct M_CORRECT as [[ub_ms' [msg M_UB]] | M_CORRECT].
-    { (* UB *)
-      left.
-      exists ub_ms'. exists msg.
-      left; auto.
-    }
+    (* unfold exec_correct in *. *)
+    (* intros ms st VALID PRE. *)
+    (* specialize (M_CORRECT ms st VALID PRE). *)
+    (* destruct M_CORRECT as [[ub_ms' [msg M_UB]] | M_CORRECT]. *)
+    (* { (* UB *) *)
+    (*   left. *)
+    (*   exists ub_ms'. exists msg. *)
+    (*   left; auto. *)
+    (* } *)
 
-    destruct M_CORRECT as [e [st' [ms' [M_EXEC_CORRECT [M_SPEC_CORRECT M_POST]]]]].
-    destruct e as [[[[[[[oom_e] | [[ub_e] | [[err_e] | e']]]]]]]] eqn:He.
+    (* destruct M_CORRECT as [e [st' [ms' [M_EXEC_CORRECT [M_SPEC_CORRECT M_POST]]]]]. *)
+    (* destruct e as [[[[[[[oom_e] | [[ub_e] | [[err_e] | e']]]]]]]] eqn:He. *)
 
-    - (* OOM *)
-      right.
-      exists (raise_oom oom_e).
-      exists st'.
-      exists ms'.
+    (* - (* OOM *) *)
+    (*   right. *)
+    (*   exists (raise_oom oom_e). *)
+    (*   exists st'. *)
+    (*   exists ms'. *)
 
-      split.
-      { (* Exec *)
-        cbn in M_EXEC_CORRECT.
-        red in M_EXEC_CORRECT.
-        cbn. red.
-        destruct M_EXEC_CORRECT as [m2 [[oom_msg OOM] EXEC]].
-        exists (raise_oom oom_msg).
-        split.
-        cbn.
-        eexists; reflexivity.
-        cbn.
-        cbn in EXEC.
-        rewrite MemMonad_run_bind.
-        rewrite EXEC.
-        rewrite OOM.
-        repeat rewrite (@rbm_raise_bind _ _ _ _ (@raise_oom _ _) _).
-        reflexivity.
-      }
+    (*   split. *)
+    (*   { (* Exec *) *)
+    (*     cbn in M_EXEC_CORRECT. *)
+    (*     red in M_EXEC_CORRECT. *)
+    (*     cbn. red. *)
+    (*     destruct M_EXEC_CORRECT as [m2 [[oom_msg OOM] EXEC]]. *)
+    (*     exists (raise_oom oom_msg). *)
+    (*     split. *)
+    (*     cbn. *)
+    (*     eexists; reflexivity. *)
+    (*     cbn. *)
+    (*     cbn in EXEC. *)
+    (*     rewrite MemMonad_run_bind. *)
+    (*     rewrite EXEC. *)
+    (*     rewrite OOM. *)
+    (*     repeat rewrite (@rbm_raise_bind _ _ _ _ (@raise_oom _ _) _). *)
+    (*     reflexivity. *)
+    (*   } *)
 
-      split.
-      { (* In spec *)
-        cbn.
-        left.
-        apply M_SPEC_CORRECT.
-      }
+    (*   split. *)
+    (*   { (* In spec *) *)
+    (*     cbn. *)
+    (*     left. *)
+    (*     apply M_SPEC_CORRECT. *)
+    (*   } *)
 
-      intros [x CONTRA].
-      inv CONTRA.
-    - (* UB *)
-      left.
-      exists ms'. exists ub_e.
-      cbn.
-      left.
-      apply M_SPEC_CORRECT.
-    - (* Err *)
-      right.
-      exists (raise_error err_e).
-      exists st'.
-      exists ms'.
+    (*   intros [x CONTRA]. *)
+    (*   inv CONTRA. *)
+    (* - (* UB *) *)
+    (*   left. *)
+    (*   exists ms'. exists ub_e. *)
+    (*   cbn. *)
+    (*   left. *)
+    (*   apply M_SPEC_CORRECT. *)
+    (* - (* Err *) *)
+    (*   right. *)
+    (*   exists (raise_error err_e). *)
+    (*   exists st'. *)
+    (*   exists ms'. *)
 
-      split.
-      { (* Exec *)
-        cbn in M_EXEC_CORRECT.
-        red in M_EXEC_CORRECT.
-        cbn. red.
-        destruct M_EXEC_CORRECT as [m2 [[err_msg ERR] EXEC]].
-        exists (raise_error err_msg).
-        split.
-        cbn.
-        eexists; reflexivity.
-        cbn.
-        cbn in EXEC.
-        rewrite MemMonad_run_bind.
-        rewrite EXEC.
-        rewrite ERR.
-        repeat rewrite (@rbm_raise_bind _ _ _ _ (@raise_error _ _) _).
-        reflexivity.
-      }
+    (*   split. *)
+    (*   { (* Exec *) *)
+    (*     cbn in M_EXEC_CORRECT. *)
+    (*     red in M_EXEC_CORRECT. *)
+    (*     cbn. red. *)
+    (*     destruct M_EXEC_CORRECT as [m2 [[err_msg ERR] EXEC]]. *)
+    (*     exists (raise_error err_msg). *)
+    (*     split. *)
+    (*     cbn. *)
+    (*     eexists; reflexivity. *)
+    (*     cbn. *)
+    (*     cbn in EXEC. *)
+    (*     rewrite MemMonad_run_bind. *)
+    (*     rewrite EXEC. *)
+    (*     rewrite ERR. *)
+    (*     repeat rewrite (@rbm_raise_bind _ _ _ _ (@raise_error _ _) _). *)
+    (*     reflexivity. *)
+    (*   } *)
 
-      split.
-      { (* In spec *)
-        cbn.
-        left.
-        apply M_SPEC_CORRECT.
-      }
+    (*   split. *)
+    (*   { (* In spec *) *)
+    (*     cbn. *)
+    (*     left. *)
+    (*     apply M_SPEC_CORRECT. *)
+    (*   } *)
 
-      intros [x CONTRA].
-      cbn in CONTRA.
-      inv CONTRA.
-    - (* Success *)
-      (* Need to know if there's UB in K... *)
-      rename e' into a.
-      forward M_POST.
-      { eexists; reflexivity. }
-      destruct M_POST as (VALID' & POST').
-      destruct POST' as (?&?&POST').
-      inv H.
-      rename x into a.
+    (*   intros [x CONTRA]. *)
+    (*   cbn in CONTRA. *)
+    (*   inv CONTRA. *)
+    (* - (* Success *) *)
+    (*   (* Need to know if there's UB in K... *) *)
+    (*   rename e' into a. *)
+    (*   forward M_POST. *)
+    (*   { eexists; reflexivity. } *)
+    (*   destruct M_POST as (VALID' & POST'). *)
+    (*   destruct POST' as (?&?&POST'). *)
+    (*   inv H. *)
+    (*   rename x into a. *)
 
-      specialize (K_CORRECT a ms ms' st st').
-      forward K_CORRECT; eauto.
-      forward K_CORRECT; eauto.
+    (*   specialize (K_CORRECT a ms ms' st st'). *)
+    (*   forward K_CORRECT; eauto. *)
+    (*   forward K_CORRECT; eauto. *)
 
-      forward K_CORRECT.
-      { cbn in M_EXEC_CORRECT.
-        red in M_EXEC_CORRECT.
-        destruct M_EXEC_CORRECT as [m2 [SUCC EXEC]].
-        cbn in *.
-        rewrite EXEC, SUCC.
-        rewrite bind_ret_l.
-        reflexivity.
-      }
+    (*   forward K_CORRECT. *)
+    (*   { cbn in M_EXEC_CORRECT. *)
+    (*     red in M_EXEC_CORRECT. *)
+    (*     destruct M_EXEC_CORRECT as [m2 [SUCC EXEC]]. *)
+    (*     Set Printing Implicit. *)
+    (*     cbn in *. *)
+    (*     rewrite EXEC, SUCC. *)
+    (*     pose proof *)
+    (*       (@bind_ret_l (ctree Eff B) (@MemMonad_eq1_runm MemM (ctree Eff B) MM MRun MPROV MSID MMS MERR MUB MOOM RunERR RunUB RunOOM EQM EQRI MLAWS MEMM) *)
+    (*          MRun _ _ *)
+    (*          (prod store_id (prod MemState X)) *)
+    (*          (fun a0 => *)
+    (*             @ret (ctree Eff B) MRun _ (st', (ms', a0))) *)
+    (*          a). *)
+    (*     cbn in *. *)
+    (*     Set Printing Implicit. *)
 
-      specialize (K_CORRECT _ _ VALID').
-      forward K_CORRECT.
-      { split; auto. }
+    (*     unfold ret in H. *)
+    (*     cbn in *. *)
+    (*     setoid_rewrite <- bind_ret_l. *)
+    (*     setoid_rewrite H. *)
+    (*     rewrite bind_ret_l. *)
+    (*     reflexivity. *)
+    (*   } *)
 
-      destruct K_CORRECT as [[ub_ms [ub_msg K_UB]] | K_CORRECT].
-      { (* UB in K *)
-        left.
-        exists ub_ms. exists ub_msg.
-        right.
-        exists ms'. exists a.
-        split; auto.
-      }
+    (*   specialize (K_CORRECT _ _ VALID'). *)
+    (*   forward K_CORRECT. *)
+    (*   { split; auto. } *)
 
-      (* UB not necessarily in K *)
-      right.
-      destruct K_CORRECT as [eb [st'' [ms'' [K_EXEC [K_SPEC K_POST]]]]].
+    (*   destruct K_CORRECT as [[ub_ms [ub_msg K_UB]] | K_CORRECT]. *)
+    (*   { (* UB in K *) *)
+    (*     left. *)
+    (*     exists ub_ms. exists ub_msg. *)
+    (*     right. *)
+    (*     exists ms'. exists a. *)
+    (*     split; auto. *)
+    (*   } *)
 
-      cbn in M_EXEC_CORRECT.
-      red in M_EXEC_CORRECT.
+    (*   (* UB not necessarily in K *) *)
+    (*   right. *)
+    (*   destruct K_CORRECT as [eb [st'' [ms'' [K_EXEC [K_SPEC K_POST]]]]]. *)
 
-      cbn in K_EXEC.
-      red in K_EXEC.
+    (*   cbn in M_EXEC_CORRECT. *)
+    (*   red in M_EXEC_CORRECT. *)
 
-      destruct M_EXEC_CORRECT as [tm [M_SUCC M_EXEC]].
-      destruct K_EXEC as [tk [K_SUCC K_EXEC]].
+    (*   cbn in K_EXEC. *)
+    (*   red in K_EXEC. *)
 
-      cbn in M_SUCC, M_EXEC.
-      rewrite M_SUCC in M_EXEC.
-      rewrite bind_ret_l in M_EXEC.
+    (*   destruct M_EXEC_CORRECT as [tm [M_SUCC M_EXEC]]. *)
+    (*   destruct K_EXEC as [tk [K_SUCC K_EXEC]]. *)
 
-      exists eb. exists st''. exists ms''.
-      split; [| split].
+    (*   cbn in M_SUCC, M_EXEC. *)
+    (*   rewrite M_SUCC in M_EXEC. *)
+    (*   rewrite bind_ret_l in M_EXEC. *)
 
-      { (* Exec *)
-        exists tk.
-        split; auto.
+    (*   exists eb. exists st''. exists ms''. *)
+    (*   split; [| split]. *)
 
-        cbn.
-        rewrite MemMonad_run_bind.
+    (*   { (* Exec *) *)
+    (*     exists tk. *)
+    (*     split; auto. *)
 
-        rewrite M_EXEC.
-        rewrite bind_ret_l.
-        rewrite K_EXEC.
-        reflexivity.
-      }
+    (*     cbn. *)
+    (*     rewrite MemMonad_run_bind. *)
 
-      { (* Spec *)
-        (* TODO: Probably a good bind lemma for this *)
-        destruct eb as [[[[[[[oom_eb] | [[ub_eb] | [[err_eb] | eb']]]]]]]] eqn:Heb;
-          try right; cbn; exists ms'; exists a; split; auto.
-      }
+    (*     rewrite M_EXEC. *)
+    (*     rewrite bind_ret_l. *)
+    (*     rewrite K_EXEC. *)
+    (*     reflexivity. *)
+    (*   } *)
 
-      { (* Post *)
-        intros [x RET].
-        subst.
-        forward K_POST; eauto.
-        destruct K_POST.
-        split; eauto.
-        exists x.
-        split; auto.
-        destruct H0 as (?&?&?).
-        inv H0.
+    (*   { (* Spec *) *)
+    (*     (* TODO: Probably a good bind lemma for this *) *)
+    (*     destruct eb as [[[[[[[oom_eb] | [[ub_eb] | [[err_eb] | eb']]]]]]]] eqn:Heb; *)
+    (*       try right; cbn; exists ms'; exists a; split; auto. *)
+    (*   } *)
 
-        repeat red.
-        exists a, ms', st'.
-        split; eauto.
-      }
-  Qed.
+    (*   { (* Post *) *)
+    (*     intros [x RET]. *)
+    (*     subst. *)
+    (*     forward K_POST; eauto. *)
+    (*     destruct K_POST. *)
+    (*     split; eauto. *)
+    (*     exists x. *)
+    (*     split; auto. *)
+    (*     destruct H0 as (?&?&?). *)
+    (*     inv H0. *)
+
+    (*     repeat red. *)
+    (*     exists a, ms', st'. *)
+    (*     split; eauto. *)
+    (*   } *)
+  Admitted.
 
   Lemma exec_correct_ret :
-    forall {MemM Eff} `{MemMonad MemM (itree Eff)}
+    forall {MemM Eff B} `{MemMonad MemM (ctree Eff B)}
       {X}
       (pre : exec_correct_pre)
       (x : X),
       exec_correct pre (ret x) (ret x) (exec_correct_post_ret x).
   Proof.
-    intros MemM Eff MM MRun MPROV MSID MMS
+    intros MemM Eff B MM MRun MPROV MSID MMS
       MERR MUB MOOM RunERR RunUB RunOOM EQM EQRI
       MLAWS H X pre x.
     intros ms st VALID PRE.
@@ -4905,11 +5010,13 @@ Module Type MemoryExecMonad (LP : LLVMParams) (MP : MemoryParams LP) (MMSP : Mem
       red.
       exists (ret x).
       split.
-      - cbn. reflexivity.
+      - cbn.
+        admit.
       - cbn.
         rewrite MemMonad_run_ret.
-        rewrite bind_ret_l.
-        reflexivity.
+        admit.
+        (* rewrite bind_ret_l.
+        reflexivity. *)
     }
 
     split; cbn; auto.
@@ -4919,10 +5026,10 @@ Module Type MemoryExecMonad (LP : LLVMParams) (MP : MemoryParams LP) (MMSP : Mem
     split; eauto.
     red.
     auto.
-  Qed.
+  Admitted.
 
   Lemma exec_correct_map_monad :
-    forall {MemM Eff} `{MemMonad MemM (itree Eff)}
+    forall {MemM Eff B} `{MemMonad MemM (ctree Eff B)}
       {A B}
       xs
       (m_exec : A -> MemM B) (m_spec : A -> MemPropT MemState B)
@@ -4949,17 +5056,17 @@ Module Type MemoryExecMonad (LP : LLVMParams) (MP : MemoryParams LP) (MMSP : Mem
   Qed.
 
   Lemma exec_correct_map_monad_ :
-    forall {MemM Eff} `{MemMonad MemM (itree Eff)}
-      {A B}
-      (xs : list A)
-      (m_exec : A -> MemM B) (m_spec : A -> MemPropT MemState B)
-      (post : A -> exec_correct_post B),
+    forall {MemM Eff B} `{MemMonad MemM (ctree Eff B)}
+      {X Y}
+      (xs : list X)
+      (m_exec : X -> MemM Y) (m_spec : X -> MemPropT MemState Y)
+      (post : X -> exec_correct_post Y),
       (forall a pre, exec_correct pre (m_exec a) (m_spec a) (post a)) ->
       forall pre, exec_correct pre (map_monad_ m_exec xs) (map_monad_ m_spec xs) (map_monad_ post xs).
   Proof.
-    intros MemM Eff MM MRun SID_FRESH MPROV MSID MMS
+    intros MemM Eff B MM MRun SID_FRESH MPROV MSID MMS
       MERR MUB MOOM RunERR RunUB RunOOM EQM EQRI
-      MLAWS A B xs m_exec m_spec H0 pre post.
+      MLAWS X Y xs m_exec m_spec H0 pre post.
     eapply exec_correct_bind; auto.
     eapply exec_correct_map_monad; auto.
     intros * VALID POST RUN.
@@ -4967,10 +5074,10 @@ Module Type MemoryExecMonad (LP : LLVMParams) (MP : MemoryParams LP) (MMSP : Mem
   Qed.
 
   Lemma exec_correct_map_monad_In :
-    forall {MemM Eff} `{MemMonad MemM (itree Eff)}
-      {A B}
-      (xs : list A)
-      (m_exec : forall (x : A), In x xs -> MemM B) (m_spec : forall (x : A), In x xs -> MemPropT MemState B)
+    forall {MemM Eff B} `{MemMonad MemM (ctree Eff B)}
+      {X Y}
+      (xs : list X)
+      (m_exec : forall (x : X), In x xs -> MemM Y) (m_spec : forall (x : X), In x xs -> MemPropT MemState Y)
       post,
       (forall a pre (IN : In a xs), exec_correct pre (m_exec a IN) (m_spec a IN) (post a IN)) ->
       forall pre, exec_correct pre (map_monad_In xs m_exec) (map_monad_In xs m_spec) (map_monad_In xs post).
@@ -4991,11 +5098,11 @@ Module Type MemoryExecMonad (LP : LLVMParams) (MP : MemoryParams LP) (MMSP : Mem
   Qed.
 
   Lemma exec_correct_raise_oom :
-    forall {MemM Eff} `{MemMonad MemM (itree Eff)}
+    forall {MemM Eff B} `{MemMonad MemM (ctree Eff B)}
       {A} (msg : string),
     forall pre post, exec_correct pre (raise_oom msg) (raise_oom msg : MemPropT MemState A) post.
   Proof.
-    intros MemM Eff MM MRun MPROV MSID MMS
+    intros MemM Eff B MM MRun MPROV MSID MMS
       MERR MUB MOOM RunERR RunUB RunOOM EQM EQRI
       MLAWS H A msg pre post.
     red.
@@ -5021,11 +5128,11 @@ Module Type MemoryExecMonad (LP : LLVMParams) (MP : MemoryParams LP) (MMSP : Mem
   Qed.
 
   Lemma exec_correct_raise_error :
-    forall {MemM Eff} `{MemMonad MemM (itree Eff)}
+    forall {MemM Eff B} `{MemMonad MemM (ctree Eff B)}
       {A} (msg1 msg2 : string),
     forall pre post, exec_correct pre (raise_error msg1) (raise_error msg2 : MemPropT MemState A) post.
   Proof.
-    intros MemM Eff MM MRun MPROV MSID MMS
+    intros MemM Eff B MM MRun MPROV MSID MMS
       MERR MUB MOOM RunERR RunUB RunOOM EQM EQRI
       MLAWS H A msg1 msg2 pre post.
     red.
@@ -5051,11 +5158,11 @@ Module Type MemoryExecMonad (LP : LLVMParams) (MP : MemoryParams LP) (MMSP : Mem
   Qed.
 
   Lemma exec_correct_raise_ub :
-    forall {MemM Eff} `{MemMonad MemM (itree Eff)}
+    forall {MemM Eff B} `{MemMonad MemM (ctree Eff B)}
       {A} (msg1 msg2 : string),
     forall pre post, exec_correct pre (raise_ub msg1) (raise_ub msg2 : MemPropT MemState A) post.
   Proof.
-    intros MemM Eff MM MRun MPROV MSID MMS
+    intros MemM Eff B MM MRun MPROV MSID MMS
       MERR MUB MOOM RunERR RunUB RunOOM EQM EQRI
       MLAWS H A msg1 msg2 pre post.
 
@@ -5089,12 +5196,12 @@ Module Type MemoryExecMonad (LP : LLVMParams) (MP : MemoryParams LP) (MMSP : Mem
   Defined.
 
   Lemma exec_correct_lift_OOM :
-    forall {MemM Eff} `{MemMonad MemM (itree Eff)}
+    forall {MemM Eff B} `{MemMonad MemM (ctree Eff B)}
       {A} (m : OOM A)
       (pre : exec_correct_pre),
       exec_correct pre (lift_OOM m) (lift_OOM m) (lift_OOM m).
   Proof.
-    intros MemM Eff MM MRun MPROV MSID MMS
+    intros MemM Eff B MM MRun MPROV MSID MMS
       MERR MUB MOOM RunERR RunUB RunOOM EQM EQRI
       MLAWS H A [NOOM | OOM] pre post.
     - apply exec_correct_ret; auto.
@@ -5102,12 +5209,12 @@ Module Type MemoryExecMonad (LP : LLVMParams) (MP : MemoryParams LP) (MMSP : Mem
   Qed.
 
   Lemma exec_correct_lift_ERR_RAISE_ERROR :
-    forall {MemM Eff} `{MemMonad MemM (itree Eff)}
+    forall {MemM Eff B} `{MemMonad MemM (ctree Eff B)}
       {A} (m : ERR A)
       (pre : _ -> _ -> Prop),
       exec_correct pre (lift_ERR_RAISE_ERROR m) (lift_ERR_RAISE_ERROR m) (lift_ERR_RAISE_ERROR m).
   Proof.
-    intros MemM Eff MM MRun MPROV MSID MMS
+    intros MemM Eff B MM MRun MPROV MSID MMS
       MERR MUB MOOM RunERR RunUB RunOOM EQM EQRI
       MLAWS H A [[ERR] | NOERR] pre.
     - apply exec_correct_raise_error; auto.
@@ -5121,10 +5228,10 @@ Module Type MemoryExecMonad (LP : LLVMParams) (MP : MemoryParams LP) (MMSP : Mem
       cbn.
       exists (ret NOERR).
       split.
-      reflexivity.
+      admit.
       rewrite MemMonad_run_ret.
-      rewrite bind_ret_l.
-      reflexivity.
+      admit. (* rewrite bind_ret_l.
+      reflexivity. *)
       split; eauto.
       intros (?&?).
       inv H2.
@@ -5132,15 +5239,15 @@ Module Type MemoryExecMonad (LP : LLVMParams) (MP : MemoryParams LP) (MMSP : Mem
       exists x.
       split; eauto.
       red; auto.
-  Qed.
+  Admitted.
 
   Lemma exec_correct_lift_err_RAISE_ERROR :
-    forall {MemM Eff} `{MemMonad MemM (itree Eff)}
+    forall {MemM Eff B} `{MemMonad MemM (ctree Eff B)}
       {A} (m : err A)
       (pre : _ -> _ -> Prop),
       exec_correct pre (lift_err_RAISE_ERROR m) (lift_err_RAISE_ERROR m) (lift_err_RAISE_ERROR m).
   Proof.
-    intros MemM Eff MM MRun MPROV MSID MMS
+    intros MemM Eff B MM MRun MPROV MSID MMS
       MERR MUB MOOM RunERR RunUB RunOOM EQM EQRI
       MLAWS H A [ERR | NOERR] pre.
     - apply exec_correct_raise_error; auto.
@@ -5153,10 +5260,10 @@ Module Type MemoryExecMonad (LP : LLVMParams) (MP : MemoryParams LP) (MMSP : Mem
       cbn.
       exists (ret NOERR).
       split.
-      reflexivity.
+      admit.
       rewrite MemMonad_run_ret.
-      rewrite bind_ret_l.
-      reflexivity.
+      admit. (* rewrite bind_ret_l.
+      reflexivity. *)
       split; eauto.
       intros (?&?).
       inv H2.
@@ -5164,7 +5271,7 @@ Module Type MemoryExecMonad (LP : LLVMParams) (MP : MemoryParams LP) (MMSP : Mem
       exists x.
       split; eauto.
       red; auto.
-  Qed.
+  Admitted.
 
   Definition get_consecutive_ptrs_post len : exec_correct_post (list ADDR.addr) :=
     (fun ms st addrs ms' st' =>
@@ -5176,7 +5283,7 @@ Module Type MemoryExecMonad (LP : LLVMParams) (MP : MemoryParams LP) (MMSP : Mem
   #[global] Hint Unfold intptr_seq_post : core.
 
   Lemma exec_correct_get_consecutive_pointers :
-    forall {MemM Eff} `{MemMonad MemM (itree Eff)}
+    forall {MemM Eff B} `{MemMonad MemM (ctree Eff B)}
       len ptr,
     forall pre,
       exec_correct
@@ -5185,7 +5292,7 @@ Module Type MemoryExecMonad (LP : LLVMParams) (MP : MemoryParams LP) (MMSP : Mem
         (get_consecutive_ptrs ptr len)
         (get_consecutive_ptrs ptr len).
   Proof.
-    intros MemM Eff MM MRun MPROV MSID MMS
+    intros MemM Eff B MM MRun MPROV MSID MMS
       MERR MUB MOOM RunERR RunUB RunOOM EQM EQRI
       MLAWS H len ptr pre.
     unfold get_consecutive_ptrs.
@@ -5206,11 +5313,11 @@ Module Type MemoryExecMonad (LP : LLVMParams) (MP : MemoryParams LP) (MMSP : Mem
   Qed.
 
   Lemma exec_correct_fresh_sid :
-    forall {MemM Eff} `{MemMonad MemM (itree Eff)} pre,
+    forall {MemM Eff B} `{MemMonad MemM (ctree Eff B)} pre,
       exec_correct pre fresh_sid fresh_sid fresh_sid.
   Proof.
     red.
-    intros MemM Eff MM MRun MPROV MSID MMS
+    intros MemM Eff B MM MRun MPROV MSID MMS
       MERR MUB MOOM RunERR RunUB RunOOM EQM EQRI
       MLAWS H pre ms st H0 PRE.
     right.
@@ -5221,9 +5328,9 @@ Module Type MemoryExecMonad (LP : LLVMParams) (MP : MemoryParams LP) (MMSP : Mem
       red.
       exists (ret sid).
       split; cbn.
-      - reflexivity.
-      - rewrite EUTT, bind_ret_l.
-        reflexivity.
+      - admit.
+      - admit. (* rewrite EUTT, bind_ret_l.
+        reflexivity. *)
     }
     2: {
       intros [x RET].
@@ -5241,12 +5348,13 @@ Module Type MemoryExecMonad (LP : LLVMParams) (MP : MemoryParams LP) (MMSP : Mem
     - unfold fresh_store_id. auto.
     - unfold read_byte_preserved.
       split; red; reflexivity.
-  Qed.
+  Admitted.
 
   Section Correctness.
     Context {MemM : Type -> Type}.
     Context {Eff : Type -> Type}.
-    Context `{MM : MemMonad MemM (itree Eff)}.
+    Context {B : Type -> Type}.
+    Context `{MM : MemMonad MemM (ctree Eff B)}.
 
     Import Monad.
 
@@ -5398,7 +5506,8 @@ Module Type MemoryExecMonad (LP : LLVMParams) (MP : MemoryParams LP) (MMSP : Mem
     Qed.
 
     Lemma exec_correct_fresh_provenance :
-      forall pre, exec_correct pre fresh_provenance fresh_provenance fresh_provenance.
+      forall pre,
+        exec_correct pre fresh_provenance fresh_provenance fresh_provenance.
     Proof using Type.
       red.
       intros pre ms st H PRE.
@@ -5410,7 +5519,7 @@ Module Type MemoryExecMonad (LP : LLVMParams) (MP : MemoryParams LP) (MMSP : Mem
         red.
         exists (ret pr).
         split; cbn.
-        - reflexivity.
+        - admit.
         - rewrite EUTT, bind_ret_l.
           reflexivity.
       }
@@ -5434,8 +5543,7 @@ Module Type MemoryExecMonad (LP : LLVMParams) (MP : MemoryParams LP) (MMSP : Mem
       - eapply allocations_preserved_mem_eq; eauto.
       - eapply frame_stack_preserved_mem_eq; eauto.
       - unfold ms_get_memory in MEM; cbn in MEM. eapply Proper_heap_preserved; eauto.
-        reflexivity.
-    Qed.
+    Admitted.
   End Correctness.
 
   Hint Resolve exec_correct_ret : EXEC_CORRECT.
@@ -5479,7 +5587,8 @@ Module Type MemoryModelExecPrimitives (LP : LLVMParams) (MP : MemoryParams LP).
   Section MemoryPrimitives.
     Context {MemM : Type -> Type}.
     Context {Eff : Type -> Type}.
-    Context `{MM : MemMonad MemM (itree Eff)}.
+    Context {B : Type -> Type}.
+    Context `{MM : MemMonad MemM (ctree Eff B)}.
 
     (*** Data types *)
     Parameter initial_frame : Frame.
@@ -5488,26 +5597,26 @@ Module Type MemoryModelExecPrimitives (LP : LLVMParams) (MP : MemoryParams LP).
     (*** Primitives on memory *)
     (** Reads *)
     Parameter read_byte :
-      forall `{MemMonad MemM (itree Eff)}, addr -> MemM SByte.
+      forall `{MemMonad MemM (ctree Eff B)}, addr -> MemM SByte.
 
     (** Writes *)
     Parameter write_byte :
-      forall `{MemMonad MemM (itree Eff)}, addr -> SByte -> MemM unit.
+      forall `{MemMonad MemM (ctree Eff B)}, addr -> SByte -> MemM unit.
 
     (** Stack allocations *)
     Parameter allocate_bytes_with_pr :
-      forall `{MemMonad MemM (itree Eff)}, list SByte -> Provenance -> MemM addr.
+      forall `{MemMonad MemM (ctree Eff B)}, list SByte -> Provenance -> MemM addr.
 
     (** Frame stacks *)
-    Parameter mempush : forall `{MemMonad MemM (itree Eff)}, MemM unit.
-    Parameter mempop : forall `{MemMonad MemM (itree Eff)}, MemM unit.
+    Parameter mempush : forall `{MemMonad MemM (ctree Eff B)}, MemM unit.
+    Parameter mempop : forall `{MemMonad MemM (ctree Eff B)}, MemM unit.
 
     (** Heap operations *)
     Parameter malloc_bytes_with_pr :
-      forall `{MemMonad MemM (itree Eff)}, list SByte -> Provenance -> MemM addr.
+      forall `{MemMonad MemM (ctree Eff B)}, list SByte -> Provenance -> MemM addr.
 
     Parameter free :
-      forall `{MemMonad MemM (itree Eff)}, addr -> MemM unit.
+      forall `{MemMonad MemM (ctree Eff B)}, addr -> MemM unit.
 
     (*** Correctness *)
 
@@ -5527,10 +5636,10 @@ Module Type MemoryModelExecPrimitives (LP : LLVMParams) (MP : MemoryParams LP).
     Parameter write_byte_preserves_store_id :
       forall st ms a b st' ms' res,
         @within MemM EQM err_ub_oom (prod store_id MemState) (prod store_id MemState)
-          (@Within_err_ub_oom_MemM MemM Eff
-             (@MemMonad_eq1_runm MemM (itree Eff) MM0 MRun MPROV MSID MMS MERR MUB MOOM RunERR RunUB
-                RunOOM EQM EQRI MLAWS MM) MRun
-             (@MemMonad_eq1_runm_equiv MemM (itree Eff) MM0 MRun MPROV MSID MMS MERR MUB MOOM RunERR
+          (@Within_err_ub_oom_MemM MemM Eff B
+             (@MemMonad_eq1_runm MemM (ctree Eff B) MM0 MRun MPROV MSID MMS MERR MUB MOOM RunERR RunUB
+                RunOOM EQM EQRI MLAWS MM)
+             (@MemMonad_eq1_runm_equiv MemM (ctree Eff B) MM0 MRun MPROV MSID MMS MERR MUB MOOM RunERR
                 RunUB RunOOM EQM EQRI MLAWS MM) RunERR RunUB RunOOM MM0 MRun MPROV MSID MMS MERR MUB
              MOOM RunERR RunUB RunOOM EQM EQRI MLAWS MM) unit
           (write_byte a b) (@pair store_id MemState st ms)
@@ -5628,22 +5737,23 @@ Module Type MemoryModelExec (LP : LLVMParams) (MP : MemoryParams LP) (MMEP : Mem
   Section Handlers.
     Context {MemM : Type -> Type}.
     Context {Eff : Type -> Type}.
-    Context `{MM : MemMonad MemM (itree Eff)}.
+    Context {B : Type -> Type}.
+    Context `{MM : MemMonad MemM (ctree Eff B)}.
 
     (** Reading uvalues *)
-    Definition read_bytes `{MemMonad MemM (itree Eff)} (ptr : addr) (len : nat) : MemM (list SByte) :=
+    Definition read_bytes `{MemMonad MemM (ctree Eff B)} (ptr : addr) (len : nat) : MemM (list SByte) :=
       (* TODO: this should maybe be UB and not OOM??? *)
       ptrs <- get_consecutive_ptrs ptr len;;
 
       (* Actually perform reads *)
       map_monad (fun ptr => read_byte ptr) ptrs.
 
-    Definition read_uvalue `{MemMonad MemM (itree Eff)} (dt : dtyp) (ptr : addr) : MemM uvalue :=
+    Definition read_uvalue `{MemMonad MemM (ctree Eff B)} (dt : dtyp) (ptr : addr) : MemM uvalue :=
       bytes <- read_bytes ptr (N.to_nat (sizeof_dtyp dt));;
       lift_err_RAISE_ERROR (deserialize_sbytes bytes dt).
 
     (** Writing uvalues *)
-    Definition write_bytes `{MemMonad MemM (itree Eff)} (ptr : addr) (bytes : list SByte) : MemM unit :=
+    Definition write_bytes `{MemMonad MemM (ctree Eff B)} (ptr : addr) (bytes : list SByte) : MemM unit :=
       (* TODO: Should this be UB instead of OOM? *)
       ptrs <- get_consecutive_ptrs ptr (length bytes);;
       let ptr_bytes := zip ptrs bytes in
@@ -5651,19 +5761,19 @@ Module Type MemoryModelExec (LP : LLVMParams) (MP : MemoryParams LP) (MMEP : Mem
       (* Actually perform writes *)
       map_monad_ (fun '(ptr, byte) => write_byte ptr byte) ptr_bytes.
 
-    Definition write_uvalue `{MemMonad MemM (itree Eff)} (dt : dtyp) (ptr : addr) (uv : uvalue) : MemM unit :=
+    Definition write_uvalue `{MemMonad MemM (ctree Eff B)} (dt : dtyp) (ptr : addr) (uv : uvalue) : MemM unit :=
       bytes <- serialize_sbytes uv dt;;
       write_bytes ptr bytes.
 
     (** Allocating dtyps *)
-    Definition allocate_bytes `{MemMonad MemM (itree Eff)}
+    Definition allocate_bytes `{MemMonad MemM (ctree Eff B)}
       (init_bytes : list SByte)
       : MemM addr
       := pr <- fresh_provenance;;
          allocate_bytes_with_pr init_bytes pr.
 
     (* Need to make sure MemPropT has provenance and sids to generate the bytes. *)
-    Definition allocate_dtyp `{MemMonad MemM (itree Eff)}
+    Definition allocate_dtyp `{MemMonad MemM (ctree Eff B)}
       (dt : dtyp) (num_elements : N)
       : MemM addr
       :=
@@ -5675,12 +5785,12 @@ Module Type MemoryModelExec (LP : LLVMParams) (MP : MemoryParams LP) (MMEP : Mem
            allocate_bytes bytes.
 
     (** Malloc *)
-    Definition malloc_bytes `{MemMonad MemM (itree Eff)} (init_bytes : list SByte) : MemM addr :=
+    Definition malloc_bytes `{MemMonad MemM (ctree Eff B)} (init_bytes : list SByte) : MemM addr :=
       pr <- fresh_provenance;;
       malloc_bytes_with_pr init_bytes pr.
 
     (** Handle memcpy *)
-    Definition memcpy `{MemMonad MemM (itree Eff)} (src dst : addr) (len : Z) (volatile : bool) : MemM unit :=
+    Definition memcpy `{MemMonad MemM (ctree Eff B)} (src dst : addr) (len : Z) (volatile : bool) : MemM unit :=
       if Z.ltb len 0
       then
         raise_ub "memcpy given negative length."
@@ -5700,7 +5810,7 @@ Module Type MemoryModelExec (LP : LLVMParams) (MP : MemoryParams LP) (MMEP : Mem
           raise_ub "memcpy with overlapping or non-equal src and dst memory locations.".
 
     (** memset spec *)
-    Definition memset `{MemMonad MemM (itree Eff)}
+    Definition memset `{MemMonad MemM (ctree Eff B)}
       (dst : addr) (val : int8) (len : Z) (sid : store_id) (volatile : bool) : MemM unit :=
       if Z.ltb len 0
       then
@@ -5709,7 +5819,7 @@ Module Type MemoryModelExec (LP : LLVMParams) (MP : MemoryParams LP) (MMEP : Mem
         let byte := uvalue_sbyte (@UVALUE_I 8 val) (DTYPE_I 8) 0 sid in
         write_bytes dst (repeatN (Z.to_N len) byte).
 
-    Definition handle_memory `{MemMonad MemM (itree Eff)} : MemoryE ~> MemM
+    Definition handle_memory `{MemMonad MemM (ctree Eff B)} : MemoryE ~> MemM
       := fun T m =>
            match m with
            (* Unimplemented *)
@@ -5736,7 +5846,7 @@ Module Type MemoryModelExec (LP : LLVMParams) (MP : MemoryParams LP) (MMEP : Mem
                end
            end.
 
-    Definition handle_memcpy `{MemMonad MemM (itree Eff)} (args : list dvalue) : MemM unit :=
+    Definition handle_memcpy `{MemMonad MemM (ctree Eff B)} (args : list dvalue) : MemM unit :=
       match args with
       | DVALUE_Addr dst ::
                     DVALUE_Addr src ::
@@ -5751,11 +5861,11 @@ Module Type MemoryModelExec (LP : LLVMParams) (MP : MemoryParams LP) (MMEP : Mem
       | _ => raise_error "Unsupported arguments to memcpy."
       end.
 
-    Definition handle_memset `{MemMonad MemM (itree Eff)} (args : list dvalue) : MemM unit.
+    Definition handle_memset `{MemMonad MemM (ctree Eff B)} (args : list dvalue) : MemM unit.
       refine
         (match args with
          | DVALUE_Addr dst ::
-             @DVALUE_I sz_val val ::
+             @DVALUE_I sz_val value ::
              @DVALUE_I sz_len len ::
              @DVALUE_I sz_vol volatile :: [] (* volatile ignored *)  =>
              _
@@ -5764,11 +5874,11 @@ Module Type MemoryModelExec (LP : LLVMParams) (MP : MemoryParams LP) (MMEP : Mem
       destruct (Pos.eq_dec sz_val 8); subst.
       - exact
           (sid <- fresh_sid;;
-           memset dst val (unsigned len) sid (equ volatile VellvmIntegers.one)).
+           memset dst value (unsigned len) sid (equ volatile VellvmIntegers.one)).
       - exact (raise_error "Unsupported arguments to memset.").
     Defined.
 
-    Definition handle_malloc `{MemMonad MemM (itree Eff)} (args : list dvalue) : MemM addr :=
+    Definition handle_malloc `{MemMonad MemM (ctree Eff B)} (args : list dvalue) : MemM addr :=
       match args with
       | [@DVALUE_I bitwidth sz] =>
           sid <- fresh_sid;;
@@ -5781,14 +5891,14 @@ Module Type MemoryModelExec (LP : LLVMParams) (MP : MemoryParams LP) (MMEP : Mem
       | _ => raise_error "Malloc: invalid arguments."
       end.
 
-    Definition handle_free `{MemMonad MemM (itree Eff)} (args : list dvalue) : MemM unit :=
+    Definition handle_free `{MemMonad MemM (ctree Eff B)} (args : list dvalue) : MemM unit :=
       match args with
       | [DVALUE_Addr ptr] =>
           free ptr
       | _ => raise_error "Free: invalid arguments."
       end.
 
-    Definition handle_intrinsic `{MemMonad MemM (itree Eff)} : IntrinsicE ~> MemM
+    Definition handle_intrinsic `{MemMonad MemM (ctree Eff B)} : IntrinsicE ~> MemM
       := fun T e =>
            match e with
            | Intrinsic t name args =>
@@ -5847,7 +5957,8 @@ Module MemoryModelTheory (LP : LLVMParams) (MP : MemoryParams LP) (MMEP : Memory
   Section Correctness.
     Context {MemM : Type -> Type}.
     Context {Eff : Type -> Type}.
-    Context `{MM : MemMonad MemM (itree Eff)}.
+    Context {B : Type -> Type}.
+    Context `{MM : MemMonad MemM (ctree Eff B)}.
 
     Import Monad.
 
@@ -6060,17 +6171,17 @@ Module MemoryModelTheory (LP : LLVMParams) (MP : MemoryParams LP) (MMEP : Memory
     Qed.
 
     Lemma read_uvalue_correct :
-      forall dt ptr pre,
-        exec_correct pre (read_uvalue dt ptr) (read_uvalue_spec dt ptr)
-          (a0 <-
-             (_ <- get_consecutive_ptrs ptr (N.to_nat (LP.SIZEOF.sizeof_dtyp dt));;
-              (fun (ms0 : MemState) (st0 : store_id) (bytes : list MP.BYTE_IMPL.SByte) 
-                 (ms'0 : MemState) (st'0 : store_id) =>
-                 Forall
-                   (fun byte : MP.BYTE_IMPL.SByte =>
-                      exists s : store_id, MemByte.sbyte_sid byte = inr s /\ s < st0) bytes /\
-                   ms0 = ms'0 /\ st0 = st'0));;
-           (fun a1 : list MP.BYTE_IMPL.SByte => lift_err_RAISE_ERROR (deserialize_sbytes a1 dt)) a0).
+      forall (dt : dtyp) (ptr : LP.ADDR.addr) (pre : exec_correct_pre),
+        @exec_correct _ _ _ _ _ _ _ _ _ _ _ _ _ _ _ _ _ _ _ pre (read_uvalue dt ptr) (read_uvalue_spec dt ptr)
+          (((a0 <-
+               ((_ <- (get_consecutive_ptrs ptr (N.to_nat (LP.SIZEOF.sizeof_dtyp dt)) : exec_correct_post _ );;
+                (fun (ms0 : MemState) (st0 : store_id) (bytes : list MP.BYTE_IMPL.SByte) 
+                   (ms'0 : MemState) (st'0 : store_id) =>
+                   Forall
+                     (fun byte : MP.BYTE_IMPL.SByte =>
+                        exists s : store_id, MemByte.sbyte_sid byte = inr s /\ s < st0) bytes /\
+                     ms0 = ms'0 /\ st0 = st'0)) : exec_correct_post (list MP.BYTE_IMPL.SByte));;
+            (fun a1 : list MP.BYTE_IMPL.SByte => lift_err_RAISE_ERROR (deserialize_sbytes a1 dt)) a0)) : exec_correct_post uvalue).
     Proof using Type.
       intros dt ptr pre.
       eapply exec_correct_bind.
@@ -6127,7 +6238,6 @@ Module MemoryModelTheory (LP : LLVMParams) (MP : MemoryParams LP) (MMEP : Memory
           rewrite MemMonad_run_raise_error.
           rewrite rbm_raise_bind; eauto.
           rewrite rbm_raise_bind; eauto.
-          reflexivity.
         + cbn.
           rewrite MemMonad_run_bind.
           rewrite MemMonad_run_ret.
@@ -6148,20 +6258,19 @@ Module MemoryModelTheory (LP : LLVMParams) (MP : MemoryParams LP) (MMEP : Memory
         rewrite bind_bind.
         rewrite rbm_raise_bind; eauto.
         rewrite rbm_raise_bind; eauto.
-        reflexivity.
     Qed.
 
     Lemma exec_correct_step_map_monad_In :
-      forall {A B}
+      forall {X Y}
         xs
-        (m_exec : forall (x : A), In x xs -> MemM B) (m_spec : forall (x : A), In x xs -> MemPropT MemState B)
+        (m_exec : forall (x : X), In x xs -> MemM Y) (m_spec : forall (x : X), In x xs -> MemPropT MemState Y)
         (pre : exec_correct_pre)
-        (post_b : forall x : A, In x xs -> exec_correct_post B)
+        (post_b : forall x : X, In x xs -> exec_correct_post Y)
         (POST_STEP :
           forall ms_init st_init a b ms st IN,
-            (@eq1 (itree Eff)
-              (@MemMonad_eq1_runm MemM (itree Eff) MM0 MRun MPROV MSID MMS MERR MUB MOOM RunERR RunUB
-                 RunOOM EQM EQRI MLAWS MM) (prod store_id (prod MemState B))
+            (@eq1 (ctree Eff B)
+              (@MemMonad_eq1_runm MemM (ctree Eff B) MM0 MRun MPROV MSID MMS MERR MUB MOOM RunERR RunUB
+                 RunOOM EQM EQRI MLAWS MM) (prod store_id (prod MemState Y))
               (MemMonad_run (m_exec a IN) ms_init st_init) (ret (st, (ms, b))))%monad ->
           post_b a IN ms_init st_init b ms st)
         (STEP :
@@ -6169,14 +6278,14 @@ Module MemoryModelTheory (LP : LLVMParams) (MP : MemoryParams LP) (MMEP : Memory
             pre ms_init st_init ->
             forall (ms : MemState) (st : store_id) a (IN : In a xs) res,
               (@within MemM EQM err_ub_oom (prod store_id MemState) (prod store_id MemState)
-                 (@Within_err_ub_oom_MemM MemM Eff
-                    (@MemMonad_eq1_runm MemM (itree Eff) MM0 MRun MPROV MSID MMS MERR MUB MOOM RunERR
-                       RunUB RunOOM EQM EQRI MLAWS MM) MRun
-                    (@MemMonad_eq1_runm_equiv MemM (itree Eff) MM0 MRun MPROV MSID MMS MERR MUB MOOM
+                 (@Within_err_ub_oom_MemM MemM Eff B
+                    (@MemMonad_eq1_runm MemM (ctree Eff B) MM0 MRun MPROV MSID MMS MERR MUB MOOM RunERR
+                       RunUB RunOOM EQM EQRI MLAWS MM)
+                    (@MemMonad_eq1_runm_equiv MemM (ctree Eff B) MM0 MRun MPROV MSID MMS MERR MUB MOOM
                        RunERR RunUB RunOOM EQM EQRI MLAWS MM) RunERR RunUB RunOOM MM0 MRun MPROV MSID
-                    MMS MERR MUB MOOM RunERR RunUB RunOOM EQM EQRI MLAWS MM) B
+                    MMS MERR MUB MOOM RunERR RunUB RunOOM EQM EQRI MLAWS MM) Y
                  (m_exec a IN) (@pair store_id MemState st_init ms_init)
-                 (@ret err_ub_oom (@Monad_err_ub_oom IdentityMonad.ident IdentityMonad.Monad_ident) B
+                 (@ret err_ub_oom (@Monad_err_ub_oom IdentityMonad.ident IdentityMonad.Monad_ident) Y
                     res) (@pair store_id MemState st ms)) /\
                 (post_b a IN) ms_init st_init res ms st /\
                 m_spec a IN ms_init (ret (ms, res)) ->
@@ -6220,25 +6329,26 @@ Module MemoryModelTheory (LP : LLVMParams) (MP : MemoryParams LP) (MMEP : Memory
           destruct H0 as (?&?&?).
           cbn in *.
           rewrite H0 in H2.
-          rewrite bind_ret_l in H2.
+          (* rewrite bind_ret_l in H2. *)
           eapply POST_STEP; eauto.
+          admit.
         }
 
         intros * VALID2 POST2 RUN2.
         apply exec_correct_ret.
-    Qed.
+    Admitted.
 
     Lemma exec_correct_step_map_monad :
-      forall {A B}
+      forall {X Y}
         xs
-        (m_exec : A -> MemM B) (m_spec : A -> MemPropT MemState B)
+        (m_exec : X -> MemM Y) (m_spec : X -> MemPropT MemState Y)
         (pre : exec_correct_pre)
-        (post_b : A -> exec_correct_post B)
+        (post_b : X -> exec_correct_post Y)
         (POST_STEP :
           forall ms_init st_init a b ms st,
-            (@eq1 (itree Eff)
-              (@MemMonad_eq1_runm MemM (itree Eff) MM0 MRun MPROV MSID MMS MERR MUB MOOM RunERR RunUB
-                 RunOOM EQM EQRI MLAWS MM) (prod store_id (prod MemState B))
+            (@eq1 (ctree Eff B)
+              (@MemMonad_eq1_runm MemM (ctree Eff B) MM0 MRun MPROV MSID MMS MERR MUB MOOM RunERR RunUB
+                 RunOOM EQM EQRI MLAWS MM) (prod store_id (prod MemState Y))
               (MemMonad_run (m_exec a) ms_init st_init) (ret (st, (ms, b))))%monad ->
           post_b a ms_init st_init b ms st)
         (STEP :
@@ -6246,14 +6356,14 @@ Module MemoryModelTheory (LP : LLVMParams) (MP : MemoryParams LP) (MMEP : Memory
             pre ms_init st_init ->
             forall (ms : MemState) (st : store_id) a res,
               (@within MemM EQM err_ub_oom (prod store_id MemState) (prod store_id MemState)
-                 (@Within_err_ub_oom_MemM MemM Eff
-                    (@MemMonad_eq1_runm MemM (itree Eff) MM0 MRun MPROV MSID MMS MERR MUB MOOM RunERR
-                       RunUB RunOOM EQM EQRI MLAWS MM) MRun
-                    (@MemMonad_eq1_runm_equiv MemM (itree Eff) MM0 MRun MPROV MSID MMS MERR MUB MOOM
+                 (@Within_err_ub_oom_MemM MemM Eff B
+                    (@MemMonad_eq1_runm MemM (ctree Eff B) MM0 MRun MPROV MSID MMS MERR MUB MOOM RunERR
+                       RunUB RunOOM EQM EQRI MLAWS MM)
+                    (@MemMonad_eq1_runm_equiv MemM (ctree Eff B) MM0 MRun MPROV MSID MMS MERR MUB MOOM
                        RunERR RunUB RunOOM EQM EQRI MLAWS MM) RunERR RunUB RunOOM MM0 MRun MPROV MSID
-                    MMS MERR MUB MOOM RunERR RunUB RunOOM EQM EQRI MLAWS MM) B
+                    MMS MERR MUB MOOM RunERR RunUB RunOOM EQM EQRI MLAWS MM) Y
                  (m_exec a) (@pair store_id MemState st_init ms_init)
-                 (@ret err_ub_oom (@Monad_err_ub_oom IdentityMonad.ident IdentityMonad.Monad_ident) B
+                 (@ret err_ub_oom (@Monad_err_ub_oom IdentityMonad.ident IdentityMonad.Monad_ident) Y
                     res) (@pair store_id MemState st ms)) /\
                 (post_b a) ms_init st_init res ms st /\
                 m_spec a ms_init (ret (ms, res)) ->
@@ -6295,25 +6405,26 @@ Module MemoryModelTheory (LP : LLVMParams) (MP : MemoryParams LP) (MMEP : Memory
           destruct H0 as (?&?&?).
           cbn in *.
           rewrite H0 in H2.
-          rewrite bind_ret_l in H2.
+          (* rewrite bind_ret_l in H2. *)
           eapply POST_STEP; eauto.
+          admit.
         }
 
         intros * VALID2 POST2 RUN2.
         apply exec_correct_ret.
-    Qed.
+    Admitted.
 
     Lemma exec_correct_step_map_monad_ :
-      forall {A B}
+      forall {X Y}
         xs
-        (m_exec : A -> MemM B) (m_spec : A -> MemPropT MemState B)
+        (m_exec : X -> MemM Y) (m_spec : X -> MemPropT MemState Y)
         (pre : exec_correct_pre)
-        (post_b : A -> exec_correct_post B)
+        (post_b : X -> exec_correct_post Y)
         (POST_STEP :
           forall ms_init st_init a b ms st,
-            (@eq1 (itree Eff)
-              (@MemMonad_eq1_runm MemM (itree Eff) MM0 MRun MPROV MSID MMS MERR MUB MOOM RunERR RunUB
-                 RunOOM EQM EQRI MLAWS MM) (prod store_id (prod MemState B))
+            (@eq1 (ctree Eff B)
+              (@MemMonad_eq1_runm MemM (ctree Eff B) MM0 MRun MPROV MSID MMS MERR MUB MOOM RunERR RunUB
+                 RunOOM EQM EQRI MLAWS MM) (prod store_id (prod MemState Y))
               (MemMonad_run (m_exec a) ms_init st_init) (ret (st, (ms, b))))%monad ->
           post_b a ms_init st_init b ms st)
         (STEP :
@@ -6321,14 +6432,14 @@ Module MemoryModelTheory (LP : LLVMParams) (MP : MemoryParams LP) (MMEP : Memory
             pre ms_init st_init ->
             forall (ms : MemState) (st : store_id) a res,
               (@within MemM EQM err_ub_oom (prod store_id MemState) (prod store_id MemState)
-                 (@Within_err_ub_oom_MemM MemM Eff
-                    (@MemMonad_eq1_runm MemM (itree Eff) MM0 MRun MPROV MSID MMS MERR MUB MOOM RunERR
-                       RunUB RunOOM EQM EQRI MLAWS MM) MRun
-                    (@MemMonad_eq1_runm_equiv MemM (itree Eff) MM0 MRun MPROV MSID MMS MERR MUB MOOM
+                 (@Within_err_ub_oom_MemM MemM Eff B
+                    (@MemMonad_eq1_runm MemM (ctree Eff B) MM0 MRun MPROV MSID MMS MERR MUB MOOM RunERR
+                       RunUB RunOOM EQM EQRI MLAWS MM)
+                    (@MemMonad_eq1_runm_equiv MemM (ctree Eff B) MM0 MRun MPROV MSID MMS MERR MUB MOOM
                        RunERR RunUB RunOOM EQM EQRI MLAWS MM) RunERR RunUB RunOOM MM0 MRun MPROV MSID
-                    MMS MERR MUB MOOM RunERR RunUB RunOOM EQM EQRI MLAWS MM) B
+                    MMS MERR MUB MOOM RunERR RunUB RunOOM EQM EQRI MLAWS MM) Y
                  (m_exec a) (@pair store_id MemState st_init ms_init)
-                 (@ret err_ub_oom (@Monad_err_ub_oom IdentityMonad.ident IdentityMonad.Monad_ident) B
+                 (@ret err_ub_oom (@Monad_err_ub_oom IdentityMonad.ident IdentityMonad.Monad_ident) Y
                     res) (@pair store_id MemState st ms)) /\
                 (post_b a) ms_init st_init res ms st /\
                 m_spec a ms_init (ret (ms, res)) ->
@@ -6336,7 +6447,7 @@ Module MemoryModelTheory (LP : LLVMParams) (MP : MemoryParams LP) (MMEP : Memory
         (forall a, exec_correct pre (m_exec a) (m_spec a) (post_b a)) ->
         exec_correct pre (map_monad_ m_exec xs) (map_monad_ m_spec xs) (map_monad_ post_b xs).
     Proof.
-      intros A B xs m_exec m_spec pre post_b POST_STEP STEP HM.
+      intros X Y xs m_exec m_spec pre post_b POST_STEP STEP HM.
       unfold map_monad_.
       apply exec_correct_bind.
       apply exec_correct_step_map_monad; auto.
@@ -6348,10 +6459,10 @@ Module MemoryModelTheory (LP : LLVMParams) (MP : MemoryParams LP) (MMEP : Memory
     Lemma get_consecutive_ptrs_preserves_state :
       forall st ms st' ms' ptr bytes a,
         @within MemM EQM err_ub_oom (prod store_id MemState) (prod store_id MemState)
-          (@Within_err_ub_oom_MemM MemM Eff
-             (@MemMonad_eq1_runm MemM (itree Eff) MM0 MRun MPROV MSID MMS MERR MUB MOOM RunERR RunUB
-                RunOOM EQM EQRI MLAWS MM) MRun
-             (@MemMonad_eq1_runm_equiv MemM (itree Eff) MM0 MRun MPROV MSID MMS MERR MUB MOOM RunERR
+          (@Within_err_ub_oom_MemM MemM Eff B
+             (@MemMonad_eq1_runm MemM (ctree Eff B) MM0 MRun MPROV MSID MMS MERR MUB MOOM RunERR RunUB
+                RunOOM EQM EQRI MLAWS MM)
+             (@MemMonad_eq1_runm_equiv MemM (ctree Eff B) MM0 MRun MPROV MSID MMS MERR MUB MOOM RunERR
                 RunUB RunOOM EQM EQRI MLAWS MM) RunERR RunUB RunOOM MM0 MRun MPROV MSID MMS MERR MUB
              MOOM RunERR RunUB RunOOM EQM EQRI MLAWS MM) (list ADDR.addr)
           (@get_consecutive_ptrs MemM MM0 MOOM MERR ptr (@Datatypes.length BYTE_IMPL.SByte bytes))
@@ -6366,7 +6477,7 @@ Module MemoryModelTheory (LP : LLVMParams) (MP : MemoryParams LP) (MMEP : Memory
       destruct H as (?&?&?).
       cbn in H, H0.
       rewrite H in H0.
-      rewrite bind_ret_l in H0.
+      (* rewrite bind_ret_l in H0. *)
       rewrite MemMonad_run_get_consecutive_ptrs in H0.
       unfold fmap in H0.
       cbn in H0.
@@ -6376,15 +6487,16 @@ Module MemoryModelTheory (LP : LLVMParams) (MP : MemoryParams LP) (MMEP : Memory
       { rewrite OOM in H0.
         rewrite rbm_raise_bind in H0; try typeclasses eauto.
         symmetry in H0.
-        apply MemMonad_eq1_raise_oom_inv in H0; contradiction.
+        (* apply MemMonad_eq1_raise_oom_inv in H0; contradiction. *)
+        admit.
       }
 
       rewrite GCP in H0.
       repeat rewrite bind_ret_l in H0.
-      eapply eq1_ret_ret in H0; try typeclasses eauto.
+      admit. (* eapply eq1_ret_ret in H0; try typeclasses eauto.
       inv H0.
-      auto.
-    Qed.
+      auto. *)
+    Admitted.
 
     Lemma write_bytes_correct :
       forall ptr bytes,
@@ -6440,7 +6552,6 @@ Module MemoryModelTheory (LP : LLVMParams) (MP : MemoryParams LP) (MMEP : Memory
           { intros ms st (?&?&?).
             eapply get_consecutive_ptrs_preserves_state in H2; inv H2.
             split; eauto.
-            lia.
           }
 
           eapply exec_correct_step_map_monad_In
@@ -6469,8 +6580,8 @@ Module MemoryModelTheory (LP : LLVMParams) (MP : MemoryParams LP) (MMEP : Memory
             eexists.
             split; cbn.
             reflexivity.
-            rewrite bind_ret_l.
-            apply H.
+            admit. (* rewrite bind_ret_l.
+            apply H. *)
           }
 
           (* STEP for map_monad_In *)
@@ -6487,7 +6598,7 @@ Module MemoryModelTheory (LP : LLVMParams) (MP : MemoryParams LP) (MMEP : Memory
       intros.
       cbn in H.
       auto.
-    Qed.
+    Admitted.
 
     Lemma to_ubytes_sids_bounded :
       forall uv dt sid st,
@@ -6569,14 +6680,16 @@ Module MemoryModelTheory (LP : LLVMParams) (MP : MemoryParams LP) (MMEP : Memory
         subst.
 
         rewrite H0 in H4.
-        rewrite bind_ret_l in H4.
+        (* rewrite bind_ret_l in H4. *)
         rewrite RUN in H4.
-        eapply eq1_ret_ret in H4; try typeclasses eauto.
-        inv H4.
+        (* eapply eq1_ret_ret in H4; try typeclasses eauto.
+        inv H4. *)
 
-        eapply to_ubytes_sids_bounded; lia.
+        eapply to_ubytes_sids_bounded.
+        (* lia. *)
+        admit.
       }
-    Qed.
+    Admitted.
 
     Lemma allocate_bytes_correct :
       forall bytes ,
@@ -6603,15 +6716,16 @@ Module MemoryModelTheory (LP : LLVMParams) (MP : MemoryParams LP) (MMEP : Memory
         destruct H0 as (?&?&?).
         cbn in *.
         rewrite H0 in H2.
-        rewrite bind_ret_l in H2.
+        (* rewrite bind_ret_l in H2. *)
         rewrite RUN in H2.
-        eapply eq1_ret_ret in H2; try typeclasses eauto.
-        inv H2.
+        (* eapply eq1_ret_ret in H2; try typeclasses eauto.
+        inv H2. *)
         destruct POST as (?&?&?&?); subst.
-        apply H.
+        (* apply H. *)
+        admit.
       }
       auto.
-    Qed.
+    Admitted.
 
     Hint Resolve allocate_bytes_correct : EXEC_CORRECT.
 
@@ -6621,8 +6735,8 @@ Module MemoryModelTheory (LP : LLVMParams) (MP : MemoryParams LP) (MMEP : Memory
         (post : exec_correct_post A)
         (POST_STEP :
           forall ms_init st_init res ms st,
-            (@eq1 (itree Eff)
-              (@MemMonad_eq1_runm MemM (itree Eff) MM0 MRun MPROV MSID MMS MERR MUB MOOM RunERR RunUB
+            (@eq1 (ctree Eff B)
+              (@MemMonad_eq1_runm MemM (ctree Eff B) MM0 MRun MPROV MSID MMS MERR MUB MOOM RunERR RunUB
                  RunOOM EQM EQRI MLAWS MM) (prod store_id (prod MemState A))
               (MemMonad_run m_exec ms_init st_init) (ret (st, (ms, res))))%monad ->
             post ms_init st_init res ms st)
@@ -6673,8 +6787,8 @@ Module MemoryModelTheory (LP : LLVMParams) (MP : MemoryParams LP) (MMEP : Memory
           repeat red in H0.
           destruct H0 as (?&?&?).
           cbn in *.
-          rewrite H0, bind_ret_l in H2.
-          auto.
+          admit. (* rewrite H0, bind_ret_l in H2.
+          auto. *)
         }
 
         intros ms st a ms' st' H0 H.
@@ -6689,7 +6803,7 @@ Module MemoryModelTheory (LP : LLVMParams) (MP : MemoryParams LP) (MMEP : Memory
         repeat red.
         exists x2, x3, x4.
         split; eauto.
-    Qed.
+    Admitted.
 
     Lemma exec_correct_repeatMN_Forall_simple :
       forall {A} (n : N) (m_exec : MemM A) (m_spec : MemPropT MemState A)
@@ -6729,11 +6843,12 @@ Module MemoryModelTheory (LP : LLVMParams) (MP : MemoryParams LP) (MMEP : Memory
           destruct H1 as (?&?&?).
           cbn in H3.
           cbn in H1.
-          rewrite H1, bind_ret_l in H3.
+          (* rewrite H1, bind_ret_l in H3.
           rewrite RUN in H3.
           eapply eq1_ret_ret in H3; try typeclasses eauto.
           inv H3.
-          auto.
+          auto. *)
+          admit.
         }
 
         intros ms st a ms' st' SPEC H.
@@ -6744,7 +6859,7 @@ Module MemoryModelTheory (LP : LLVMParams) (MP : MemoryParams LP) (MMEP : Memory
         destruct H as (?&?&?); subst.
         destruct H1 as (?&?&?); subst.
         auto.
-    Qed.
+    Admitted.
 
     Lemma exec_correct_clear_assertion :
       forall {A} (pre : MemState -> store_id -> Prop) (m_exec : MemM A) (m_spec : MemPropT MemState A) (assertion : Prop) post,
@@ -6788,14 +6903,14 @@ Module MemoryModelTheory (LP : LLVMParams) (MP : MemoryParams LP) (MMEP : Memory
 
     Lemma MemMonad_repeatMN_repeatN :
       forall ms st num_elements l,
-        @eq1 (itree Eff)
-          (@MemMonad_eq1_runm MemM (itree Eff) MM0 MRun MPROV MSID MMS MERR MUB MOOM RunERR RunUB
+        @eq1 (ctree Eff B)
+          (@MemMonad_eq1_runm MemM (ctree Eff B) MM0 MRun MPROV MSID MMS MERR MUB MOOM RunERR RunUB
              RunOOM EQM EQRI MLAWS MM) (prod store_id (prod MemState (list (list BYTE_IMPL.SByte))))
-          (@MemMonad_run MemM (itree Eff) MM0 MRun MPROV MSID MMS MERR MUB MOOM RunERR RunUB RunOOM EQM
+          (@MemMonad_run MemM (ctree Eff B) MM0 MRun MPROV MSID MMS MERR MUB MOOM RunERR RunUB RunOOM EQM
              EQRI MLAWS MM (list (list BYTE_IMPL.SByte))
              (@repeatMN (list BYTE_IMPL.SByte) MemM MM0 num_elements
                 (@ret MemM MM0 (list BYTE_IMPL.SByte) l)) ms st)
-          (@ret (itree Eff) MRun (prod store_id (prod MemState (list (list BYTE_IMPL.SByte))))
+          (@ret (ctree Eff B) MRun (prod store_id (prod MemState (list (list BYTE_IMPL.SByte))))
              (@pair store_id (prod MemState (list (list BYTE_IMPL.SByte))) st
                 (@pair MemState (list (list BYTE_IMPL.SByte)) ms (repeatN num_elements l)))).
     Proof.
@@ -6938,7 +7053,7 @@ Module MemoryModelTheory (LP : LLVMParams) (MP : MemoryParams LP) (MMEP : Memory
           repeat red in H0.
           destruct H0 as (?&?&?).
           cbn in H0, H2.
-          rewrite H0, bind_ret_l in H2.
+          (* rewrite H0, bind_ret_l in H2.
           rewrite RUN1 in H2.
           eapply eq1_ret_ret in H2; try typeclasses eauto.
           inv H2.
@@ -6949,7 +7064,8 @@ Module MemoryModelTheory (LP : LLVMParams) (MP : MemoryParams LP) (MMEP : Memory
 
           eapply generate_undef_bytes_bounded; eauto.
           destruct POST1 as (?&?&?); subst.
-          lia.
+          lia. *)
+          admit.
         }
 
         intros * VALID2 POST2 RUN2.
@@ -6965,7 +7081,7 @@ Module MemoryModelTheory (LP : LLVMParams) (MP : MemoryParams LP) (MMEP : Memory
           repeat red in H2.
           destruct H2 as (?&?&?).
           cbn in *.
-          rewrite H2, bind_ret_l in H6.
+          (* rewrite H2, bind_ret_l in H6.
           destruct POST1 as (?&?&?); subst.
           rewrite RUN1 in H6.
           eapply eq1_ret_ret in H6; try typeclasses eauto.
@@ -6997,10 +7113,11 @@ Module MemoryModelTheory (LP : LLVMParams) (MP : MemoryParams LP) (MMEP : Memory
             inv H5; auto.
           }
           subst.
-          auto.
+          auto. *)
+          admit.
         }
       }
-    Qed.
+    Admitted.
 
     Lemma memcpy_correct :
       forall src dst len volatile pre,
@@ -7076,13 +7193,14 @@ Module MemoryModelTheory (LP : LLVMParams) (MP : MemoryParams LP) (MMEP : Memory
         repeat red in H0.
         destruct H0 as (?&?&?).
         cbn in H0, H3.
-        rewrite H0, bind_ret_l in H3.
+        (* rewrite H0, bind_ret_l in H3.
         rewrite RUN in H3.
         eapply eq1_ret_ret in H3; try typeclasses eauto.
         inv H3.
-        auto.
+        auto. *)
+        admit.
       }
-    Qed.
+    Admitted.
 
     Lemma memset_correct :
       forall dst val len sid volatile,
@@ -7207,14 +7325,15 @@ Module MemoryModelTheory (LP : LLVMParams) (MP : MemoryParams LP) (MMEP : Memory
           repeat red in H3.
           destruct H3 as (?&?&?).
           cbn in *.
-          rewrite H3, bind_ret_l, H1 in H5.
+          (* rewrite H3, bind_ret_l, H1 in H5.
           eapply eq1_ret_ret in H5; try typeclasses eauto.
           inv H5.
-          lia.
+          lia. *)
+          admit.
         }
         auto.
       }
-    Qed.
+    Admitted.
 
     Lemma malloc_bytes_correct :
       forall bytes,
@@ -7236,16 +7355,17 @@ Module MemoryModelTheory (LP : LLVMParams) (MP : MemoryParams LP) (MMEP : Memory
         destruct H3 as (?&?&?).
         cbn in H3.
         cbn in H5.
-        rewrite H3, bind_ret_l, H1 in H5.
+        (* rewrite H3, bind_ret_l, H1 in H5.
         eapply eq1_ret_ret in H5; try typeclasses eauto.
         inv H5.
         auto.
         destruct H0 as (?&?&?&?).
         subst.
-        auto.
+        auto. *)
+        admit.
       }
       auto.
-    Qed.
+    Admitted.
 
     Hint Resolve malloc_bytes_correct : EXEC_CORRECT.
 
@@ -7284,7 +7404,7 @@ Module MemoryModelTheory (LP : LLVMParams) (MP : MemoryParams LP) (MMEP : Memory
           cbn in H3.
           cbn in H6.
           rewrite H3 in H6.
-          rewrite MemMonad_run_ret, bind_ret_l in H6.
+          (* rewrite MemMonad_run_ret, bind_ret_l in H6.
           eapply eq1_ret_ret in H6; try typeclasses eauto.
           inv H6.
           cbn in H1.
@@ -7295,7 +7415,8 @@ Module MemoryModelTheory (LP : LLVMParams) (MP : MemoryParams LP) (MMEP : Memory
           rewrite RUN in H6.
           eapply eq1_ret_ret in H6; try typeclasses eauto.
           inv H6.
-          lia.
+          lia. *)
+          admit.
         }
         
         eauto with EXEC_CORRECT.
@@ -7325,7 +7446,7 @@ Module MemoryModelTheory (LP : LLVMParams) (MP : MemoryParams LP) (MMEP : Memory
           cbn in H3.
           cbn in H6.
           rewrite H3 in H6.
-          rewrite MemMonad_run_ret, bind_ret_l in H6.
+          (* rewrite MemMonad_run_ret, bind_ret_l in H6.
           eapply eq1_ret_ret in H6; try typeclasses eauto.
           inv H6.
           cbn in H1.
@@ -7336,13 +7457,14 @@ Module MemoryModelTheory (LP : LLVMParams) (MP : MemoryParams LP) (MMEP : Memory
           rewrite RUN in H6.
           eapply eq1_ret_ret in H6; try typeclasses eauto.
           inv H6.
-          lia.
+          lia. *)
+          admit.
         }
         
         eauto with EXEC_CORRECT.
         eauto with EXEC_CORRECT.
       }
-    Qed.
+    Admitted.
 
     Lemma handle_free_correct:
       forall args pre,
@@ -7720,11 +7842,12 @@ Module MemStateInfiniteHelpers (LP : LLVMParamsBig) (MP : MemoryParams LP) (MMSP
 
       destruct IHl as (ips & IHl).
       exists (i :: ips).
-      setoid_rewrite functional_extensionality.
+      (* setoid_rewrite functional_extensionality.
       rewrite IHl.
       reflexivity.
-      reflexivity.
-  Qed.
+      reflexivity. *)
+      admit.
+  Admitted.
 
   #[global] Instance lift_err_RAISE_ERROR_Proper {A M} `{HM: Monad M} `{RAISE: RAISE_ERROR M} `{EQM : Eq1 M} `{EQV : @Eq1Equivalence M HM EQM} :
     Proper (eq ==> eq1) (@lift_err_RAISE_ERROR A M HM RAISE).
@@ -7781,10 +7904,10 @@ Module MemStateInfiniteHelpers (LP : LLVMParamsBig) (MP : MemoryParams LP) (MMSP
       reflexivity.
     }
     { apply map_monad_OOM_fail in HSEQUENCE as [a [IN EQA]].
-      unfold id in EQA. subst.
+      unfold Datatypes.id in EQA. subst.
 
       pose proof map_monad_err_In _ _ _ _ HMAPM IN as [ix [GEP INix]].
-      apply handle_gep_addr_ix_OOM in GEP; auto.
+      eapply handle_gep_addr_ix_OOM in GEP; auto.
       destruct GEP as [msg' GEP].
       pose proof
         (LP.I2P_BIG.int_to_ptr_safe (ptr_to_int ptr + Z.of_N (sizeof_dtyp (DTYPE_I 8)) * to_Z ix)
